src/cbor/pulse/raw/CBOR.Pulse.Raw.Nondet.Compare.fst
@@ -82,7 +82,7 @@ ensures
       CBOR.Spec.Util.setoid_assoc_eq SpecRaw.raw_equiv SpecRaw.raw_equiv v1 v2 == (match res with Some r -> r | _ -> CBOR.Spec.Util.setoid_assoc_eq SpecRaw.raw_equiv SpecRaw.raw_equiv l1 v2)
     )
   ) {
-    let x1 = Read.cbor_map_iterator_next () pi1;
+    let x1 = Read.cbor_map_iterator_next pi1;
     Trade.trans _ _ (Read.cbor_map_iterator_match p1 i1 v1);
     with px1 vx1 . assert (Read.cbor_match_map_entry px1 x1 vx1);
     unfold (Read.cbor_match_map_entry px1 x1 vx1);
@@ -149,7 +149,7 @@ ensures
       List.Tot.for_all (CBOR.Spec.Util.setoid_assoc_eq SpecRaw.raw_equiv SpecRaw.raw_equiv v1) v2 == (res && List.Tot.for_all (CBOR.Spec.Util.setoid_assoc_eq SpecRaw.raw_equiv SpecRaw.raw_equiv v1) l2)
     )
   ) {
-    let x2 = Read.cbor_map_iterator_next () pi2;
+    let x2 = Read.cbor_map_iterator_next pi2;
     Trade.trans _ _ (Read.cbor_map_iterator_match p2 i2 v2);
     pres := cbor_nondet_setoid_assoc_eq cbor_nondet_equiv i1 x2;
     Trade.elim_hyp_l _ _ _
@@ -282,9 +282,9 @@ fn cbor_nondet_equiv_body
             (SpecRaw.raw_equiv v1 v2 == (res && CBOR.Spec.Util.list_for_all2 SpecRaw.raw_equiv l1 l2))
           )
         ) {
-          let y1 = Read.cbor_array_iterator_next () pi1;
+          let y1 = Read.cbor_array_iterator_next pi1;
           Trade.trans _ _ (cbor_match p1 x1 v1);
-          let y2 = Read.cbor_array_iterator_next () pi2;
+          let y2 = Read.cbor_array_iterator_next pi2;
           Trade.trans _ _ (cbor_match p2 x2 v2);
           pres := cbor_nondet_equiv y1 y2;
           Trade.elim_hyp_l _ _ (cbor_match p1 x1 v1);
