src/cbor/pulse/raw/everparse/CBOR.Pulse.Raw.Format.Nondet.Validate.fst
@@ -18,7 +18,6 @@ ensures
     cbor_validate_nondet_post map_key_bound strict_check v res
   ))
 {
-  assume (pure (SZ.fits_u64));
   let mut poff = 0sz;
   let res = EP.validate_raw_data_item () input poff;
   if (res) {
